wip on specifying the opposite direction of the primitives of RiscvProgram
This will be needed by anyone who wants to consume a riscv execution

src/util/Monads.v
@@ -114,6 +114,11 @@ Module OStateOperations.
   Definition computation_satisfies{S: Type}(m: OState S unit)(s: S)(post: S -> Prop): Prop :=
     exists s', m s = (Some tt, s') /\ post s'.
 
+  (* provides the link between "S -> option A * S" and "S -> (A -> S -> Prop) -> Prop" *)
+  Definition computation_with_answer_satisfies
+             {S A: Type}(m: OState S A)(s: S)(post: A -> S -> Prop): Prop :=
+    exists a s', m s = (Some a, s') /\ post a s'.
+
 End OStateOperations.
 
 
@@ -160,6 +165,11 @@ Module OStateNDOperations.
   (* provides the link between "S -> option (A * S) -> Prop" and "S -> (S -> Prop) -> Prop" *)
   Definition computation_satisfies{S: Type}(m: OStateND S unit)(s: S)(post: S -> Prop): Prop :=
     forall (o: option (unit * S)), m s o -> exists s', o = Some (tt, s') /\ post s'.
+
+  (* provides the link between "S -> option (A * S) -> Prop" and "S -> (A -> S -> Prop) -> Prop" *)
+  Definition computation_with_answer_satisfies
+             {S A: Type}(m: OStateND S A)(s: S)(post: A -> S -> Prop): Prop :=
+    forall (o: option (A * S)), m s o -> exists a s', o = Some (a, s') /\ post a s'.
 
 End OStateNDOperations.
 
