src/Primitives.v
@@ -1,0 +1,87 @@
+Require Import Coq.Lists.List.
+Require Import Coq.ZArith.BinInt.
+Require Import coqutil.Map.Interface.
+Require Import riscv.util.Monads.
+Require Import riscv.Utility.
+Require Import riscv.Decode.
+Require Import riscv.Memory.
+Require Import riscv.Program.
+Require Import riscv.RiscvMachine.
+Require Import riscv.MkMachineWidth.
+
+
+(* Note: Register 0 is not considered valid because it cannot be written *)
+Definition valid_register(r: Register): Prop := (0 < r < 32)%Z.
+
+Section Primitives.
+
+  Context {W: Words}.
+  Context {RFF: RegisterFileFunctions Register word}.
+  Context {Action: Type}.
+  Context {mem: map.map word byte}.
+
+  Local Notation RiscvMachineL := (RiscvMachine Register Action).
+
+  Context {M: Type -> Type}.
+  Context {MM: Monad M}.
+  Context {RVM: RiscvProgram M word}.
+  Context {RVS: @RiscvState M word _ _ RVM}.
+
+  Class Primitives :=  {
+
+    (* Abstract predicate specifying when a monadic computation satisfies a
+       postcondition when run on given initial machine *)
+    mcomp_sat: forall {A: Type}, M A -> RiscvMachineL -> (A -> RiscvMachineL -> Prop) -> Prop;
+
+    spec_Bind{A B: Type}: forall (initialL: RiscvMachineL) (post: B -> RiscvMachineL -> Prop)
+                                 (m: M A) (f : A -> M B),
+        (exists mid: A -> RiscvMachineL -> Prop,
+            mcomp_sat m initialL mid /\
+            (forall a middle, mid a middle -> mcomp_sat (f a) middle post)) <->
+        mcomp_sat (Bind m f) initialL post;
+
+    spec_Return{A: Type}: forall (initialL: RiscvMachineL)
+                                 (post: A -> RiscvMachineL -> Prop) (a: A),
+        post a initialL <->
+        mcomp_sat (Return a) initialL post;
+
+    spec_getRegister: forall (initialL: RiscvMachineL) (x: Register)
+                             (post: word -> RiscvMachineL -> Prop),
+        (valid_register x /\ post (getReg initialL.(getRegs) x) initialL \/
+         x = Register0 /\ post (word.of_Z 0) initialL) <->
+        mcomp_sat (getRegister x) initialL post;
+
+    spec_setRegister: forall initialL x v (post: unit -> RiscvMachineL -> Prop),
+      (valid_register x /\ post tt (setRegs initialL (setReg initialL.(getRegs) x v)) \/
+       x = Register0 /\ post tt initialL) <->
+      mcomp_sat (setRegister x v) initialL post;
+
+    spec_loadWord: forall initialL addr (post: w32 -> RiscvMachineL -> Prop),
+        (exists v: w32,
+            Memory.loadWord initialL.(getMem) addr = Some v /\ post v initialL) <->
+        mcomp_sat (Program.loadWord (RiscvProgram := RVM) addr) initialL post;
+
+    spec_storeWord: forall initialL addr v (post: unit -> RiscvMachineL -> Prop),
+        (exists m',
+            Memory.storeWord initialL.(getMem) addr v = Some m' /\
+            post tt (withMem m' initialL)) <->
+        mcomp_sat (Program.storeWord addr v) initialL post;
+
+    spec_getPC: forall initialL (post: word -> RiscvMachineL -> Prop),
+        post initialL.(getPc) initialL <->
+        mcomp_sat getPC initialL post;
+
+    spec_setPC: forall initialL v (post: unit -> RiscvMachineL -> Prop),
+        post tt (withNextPc v initialL) <->
+        mcomp_sat (setPC v) initialL post;
+
+    spec_step: forall initialL (post: unit -> RiscvMachineL -> Prop),
+        post tt (withNextPc (word.add initialL.(getNextPc) (word.of_Z 4))
+                (withPc     initialL.(getNextPc)
+                            initialL)) <->
+        mcomp_sat step initialL post;
+  }.
+
+End Primitives.
+
+Arguments Primitives {_} {_} Action {_} M {_} {_}.
